TA_Network/NTA_Temp_Planning_Sem.thy
@@ -1,0 +1,377 @@
+theory NTA_Temp_Planning_Sem
+  imports Temporal_Planning_Base.Temporal_Plans
+begin
+
+locale nta_temp_planning = 
+  finite_props_temp_planning_problem init goal at_start at_end over_all lower upper pre adds dels \<epsilon> props actions  +
+  unique_snaps_temp_planning_problem init goal at_start at_end over_all lower upper pre adds dels \<epsilon> props actions 
+    for init::    "'proposition set"
+    and goal::    "'proposition set"
+    and at_start::"'action  \<Rightarrow> 'snap_action"
+    and at_end::  "'action  \<Rightarrow> 'snap_action"
+    and over_all::"'action  \<Rightarrow> 'proposition set"
+    and lower::   "'action  \<rightharpoonup> ('time::time) lower_bound"
+    and upper::   "'action  \<rightharpoonup> 'time upper_bound"
+    and pre::     "'snap_action \<Rightarrow> 'proposition set"
+    and adds::    "'snap_action \<Rightarrow> 'proposition set"
+    and dels::    "'snap_action \<Rightarrow> 'proposition set"
+    and \<epsilon>::       "'time"
+    and props::   "'proposition set"
+    and actions:: "'action set" 
++  
+fixes \<pi>::"('i, 'action, 'time) temp_plan"
+assumes vp: "valid_plan \<pi> init goal at_start at_end over_all lower upper pre adds dels \<epsilon>"
+    and pap: "plan_actions_in_problem \<pi> actions"
+    and nso: "no_self_overlap \<pi>"
+begin
+
+lemma at_start_inj_on_plan: 
+  assumes "pap_\<pi>"
+  shows "inj_on at_start {a| a t d. (a, t, d) \<in> ran \<pi>}"
+  using assms at_start_inj_on unfolding inj_on_def plan_actions_in_problem_def by blast
+
+lemma at_end_inj_on_plan:
+  assumes "pap_\<pi>"
+  shows "inj_on at_end {a| a t d. (a, t, d) \<in> ran \<pi>}"
+  using assms at_end_inj_on unfolding inj_on_def plan_actions_in_problem_def by blast
+
+lemma snaps_disj_on_plan:
+  assumes "pap_\<pi>"
+  shows "at_start ` {a| a t d. (a, t, d) \<in> ran \<pi>} \<inter> at_end ` {a| a t d. (a, t, d) \<in> ran \<pi>} = {}"
+  using assms snaps_disj unfolding plan_actions_in_problem_def by fast
+
+lemma at_start_in_happ_seqE':
+  assumes a_in_acts: "a \<in> actions"
+      and pap: pap_\<pi>
+      and nso: nso_\<pi>
+      and dp: dp_\<pi>
+      and sn: "(s, at_start a) \<in> plan_happ_seq \<pi> at_start at_end"
+    shows "\<exists>!(t, d). (a, t, d) \<in> ran \<pi> \<and> s = t"
+  using at_start_in_happ_seqE[OF _ at_start_inj_on at_end_inj_on snaps_disj sn a_in_acts nso]
+  using dp[THEN dp_imp_dg0] pap unfolding plan_actions_in_problem_def by auto
+
+lemma at_end_in_happ_seqE':
+  assumes a_in_acts: "a \<in> actions"
+      and pap: pap_\<pi>
+      and nso: nso_\<pi>
+      and dp: dp_\<pi>
+      and sn: "(s, at_end a) \<in> plan_happ_seq \<pi> at_start at_end"
+    shows "\<exists>!(t, d). (a, t, d) \<in> ran \<pi> \<and> s = t + d"
+  using at_end_in_happ_seqE[OF _ at_start_inj_on at_end_inj_on snaps_disj sn a_in_acts nso]
+  using dp[THEN dp_imp_dg0] pap unfolding plan_actions_in_problem_def by auto
+  
+lemma eps_cases: 
+  assumes "\<epsilon> = 0 \<Longrightarrow> thesis"
+      and "0 \<le> \<epsilon> \<Longrightarrow> thesis"
+    shows "thesis"
+  using assms eps_range by blast
+
+abbreviation snaps::"'action \<Rightarrow> 'snap_action set" where
+"snaps a \<equiv> {at_start a, at_end a}"
+
+definition snap_actions::"'snap_action set" where
+"snap_actions \<equiv> (at_start ` actions) \<union> (at_end ` actions)"
+
+
+definition "happ_seq \<equiv> plan_happ_seq \<pi> at_start at_end"
+
+definition "pap \<equiv> plan_actions_in_problem \<pi> actions"
+
+definition "dur_valid \<equiv> durations_valid \<pi> lower upper"
+
+definition "valid_state_seq \<equiv> valid_state_sequence \<pi> at_start at_end over_all pre adds dels"
+
+definition "invariant_sequence = plan_inv_seq \<pi> over_all"
+
+definition "mutex_valid_happ_seq = nm_happ_seq pre adds dels"
+
+definition "dur_bounds_sat = satisfies_duration_bounds lower upper"
+
+definition "app_effs \<equiv> apply_effects adds dels"
+
+definition "plan_state_seq \<equiv> SOME MS. valid_state_seq MS"
+
+lemma plan_state_seq_valid: "valid_state_seq plan_state_seq"
+  using vp unfolding valid_plan_def Let_def  valid_state_seq_def 
+    plan_state_seq_def 
+  unfolding valid_state_seq_def[symmetric]
+  apply -
+  apply (rule  Hilbert_Choice.someI_ex[where P = valid_state_seq])
+  by blast
+subsubsection \<open>Proposition and execution state\<close>
+
+definition exec_state_sequence::"('time \<times> 'action) set" where
+"exec_state_sequence \<equiv> {(t, a) |s t a. a \<in> actions \<and> (s, at_start a) \<in> happ_seq \<and> s < t 
+                  \<and> \<not>(\<exists>s'. (s', at_end a) \<in> happ_seq \<and> s \<le> s' \<and> s' < t)}"
+
+definition exec_state_sequence'::"('time \<times> 'action) set" where
+"exec_state_sequence' \<equiv> {(t, a) |s t a. a \<in> actions \<and> (s, at_start a) \<in> happ_seq \<and> s \<le> t 
+                  \<and> \<not>(\<exists>s'. (s', at_end a) \<in> happ_seq \<and> s \<le> s' \<and> s' \<le> t)}"
+
+abbreviation "ES t \<equiv> {a. (t, a) \<in> exec_state_sequence}"
+
+abbreviation "IES t \<equiv> {a. (t, a) \<in> exec_state_sequence'}"
+
+abbreviation "PES t \<equiv> {a. (t, at_start a) \<in> happ_seq \<and> (t, at_end a) \<in> happ_seq}" 
+
+
+lemma inc_es_is_next_es:
+  assumes "finite_\<pi>"
+      and "Suc l < length htpl"
+  shows "IES (ti l) = ES (ti(Suc l))"
+proof (rule equalityI; rule subsetI)
+  fix a
+  assume "a \<in> IES (ti l)"
+  then obtain s where
+    s: "a \<in> actions \<and> (s, at_start a) \<in> happ_seq \<and> s \<le> ti l"
+    "\<not>(\<exists>s'. (s', at_end a) \<in> happ_seq \<and> s \<le> s' \<and> s' \<le> ti l)"
+    unfolding exec_state_sequence'_def by blast
+  from this(2) time_index_strict_sorted_list[rotated, OF assms(2)] no_actions_between_indexed_timepoints[OF assms]
+  have "\<not>(\<exists>s'. (s', at_end a) \<in> happ_seq \<and> s \<le> s' \<and> s' < ti (Suc l))"
+    try0
+  with time_index_strict_sorted_list[rotated, OF \<open>Suc l < length htpl\<close>] s(1)
+  show "a \<in> ES (ti(Suc l))" using exec_state_sequence_def by force
+next
+  fix a
+  assume "a \<in> ES (ti (Suc l))"
+  then obtain s where
+    s: "a \<in> actions"
+    "(s, at_start a) \<in> happ_seq"  
+    "s < ti (Suc l)"
+    "\<not>(\<exists>s'. (s', at_end a) \<in> happ_seq \<and> s \<le> s' \<and> s' < ti (Suc l))"
+    unfolding exec_state_sequence_def by blast
+  from this(2, 3) no_actions_between_indexed_timepoints[OF assms]
+  have "s \<le> ti l" by fastforce
+  moreover
+  have "\<not>(\<exists>s'. (s', at_end a) \<in> happ_seq \<and> s \<le> s' \<and> s' \<le> ti l)" 
+  proof (rule notI)
+    assume "\<exists>s'. (s', at_end a) \<in> happ_seq \<and> s \<le> s' \<and> s' \<le> ti l"
+    with time_index_strict_sorted_list assms(2)
+    have "\<exists>s'. (s', at_end a) \<in> happ_seq \<and> s \<le> s' \<and> s' < ti(Suc l)" by fastforce
+    with s(4)
+    show "False" by blast
+  qed
+  ultimately
+  show "a \<in> IES (ti l)" using s(1,2) exec_state_sequence'_def by blast
+qed
+
+lemma last_ies_empty:
+  assumes pap: "pap_\<pi>"
+      and dnz: "dp_\<pi>"
+      and fpl:  "fp_\<pi>"
+  shows "IES (ti(length htpl - 1)) = {}" (is "IES ?te = {}")
+proof -   
+  have "a \<notin> IES ?te" for a
+  proof (rule notI)
+    assume a: "a \<in> IES ?te"
+    then obtain s where
+      s: "a \<in> actions"
+      "(s, at_start a) \<in> happ_seq" 
+      "s \<le> ?te"
+      "\<not>(\<exists>s'. (s', at_end a) \<in> happ_seq \<and> s \<le> s' \<and> s' \<le> ?te)"
+      using exec_state_sequence'_def by blast
+    from this(2)[simplified plan_happ_seq_def]
+    consider "(s, at_start a) \<in> {(t, at_start a)|a t d. (a, t, d) \<in> ran \<pi>}" 
+      | "(s, at_start a) \<in>  {(t + d, at_end a) |a t d. (a, t, d) \<in> ran \<pi>}"
+      by blast
+    then
+    have "\<exists>d. (a, s, d) \<in> ran \<pi>"
+    proof cases
+      case 1
+      hence "\<exists>a' t d. (s, at_start a) = (t, at_start a') \<and> (a', t, d) \<in> ran \<pi>" by blast
+      thus ?thesis using at_start_inj_on[simplified inj_on_def] \<open>a \<in> actions\<close> pap[simplified plan_actions_in_problem_def] by blast
+    next
+      case 2
+      hence "\<exists>a' t d. (s, at_start a) = (t + d, at_end a') \<and> (a', t, d) \<in> ran \<pi>" by auto
+      with s(1) assms(1)[simplified plan_actions_in_problem_def] snaps_disj
+      have False by blast
+      thus ?thesis ..
+    qed
+    then obtain d where
+      d: "(a, s, d) \<in> ran \<pi>"
+      "(s + d, at_end a) \<in> happ_seq" using plan_happ_seq_def by fast
+    with s(4) assms(2)[simplified durations_positive_def]
+    have "s + d > ?te" by fastforce
+    
+    have "t \<le> ?te" if "t \<in> set htpl" for t
+    proof -
+      from that[simplified time_index_bij_betw_list[simplified bij_betw_def, THEN conjunct2, symmetric]]
+      obtain n where
+        n: "n < length htpl" "t = ti n" by blast
+      show "t \<le> ?te"
+      proof (cases "n < length htpl - 1")
+        case True
+        show ?thesis
+          apply (subst n(2))
+          apply (rule time_index_sorted_list)
+          using True by simp+
+      next
+        case False
+        hence "n = length htpl - 1" using n by linarith
+        thus ?thesis using n by blast
+      qed
+    qed
+    moreover
+    
+    from d(1) set_htpl_eq_htps[OF fpl] 
+    have "s + d \<in> set htpl" unfolding htps_def by blast
+    ultimately
+    show False using \<open>s + d > ?te\<close> by fastforce
+  qed
+  thus "IES ?te = {}" by blast
+qed
+
+lemma first_es_empty:
+assumes pap: "pap_\<pi>"
+      and dnz: "dp_\<pi>"
+      and fpl:  "fp_\<pi>"
+    shows "ES (ti 0) = {}"
+proof (rule ccontr)
+  assume "ES (ti 0) \<noteq> {}"
+  then obtain a where
+    a: "a \<in> ES (ti 0)" by blast
+
+  then obtain t where
+    t: "t < ti 0"
+    "at_start a \<in> B t" using in_ES_iff by blast
+
+  show False
+  proof (cases "card timepoint_set")
+    case 0
+    with time_index_img_set fpl
+    have "timepoint_set = {}" by fastforce
+    with t(2) a_in_B_iff_t_in_htps
+    show ?thesis by fast
+  next
+    case (Suc nat)
+    hence "0 < card timepoint_set" by auto
+    from t(2)
+    have "t \<in> timepoint_set" using a_in_B_iff_t_in_htps by fast
+    then obtain i where
+      i: "t = ti i" 
+      "i < card timepoint_set" using time_index_img_set fpl by blast
+    have "0 \<le> i" by simp
+    with i(2)
+    have "ti 0 \<le> ti i" using time_index_sorted_set by blast
+    with i(1) t
+    show ?thesis by simp
+  qed
+qed
+
+lemma not_executing_when_starting:
+  assumes snap_in_B: "(at_start a) \<in> B t"
+      and a_in_actions: "a \<in> actions"
+      and no_self_overlap: "nso_\<pi>"
+      and durations_positive: "dp_\<pi>"
+      and plan_actions_in_problem: "pap_\<pi>"
+  shows "a \<notin> ES t"
+proof (rule notI)
+  assume "a \<in> ES t"
+  then obtain s where
+    started: "a \<in> actions \<and> (s, at_start a) \<in> happ_seq \<and> s < t"
+    and not_ended: "\<not>(\<exists>s'. (s', at_end a) \<in> happ_seq \<and> s \<le> s' \<and> s' < t)"
+    unfolding exec_state_sequence_def by blast
+  
+  from started
+  obtain d where
+    as_in_plan: "(a, s, d) \<in> ran \<pi>"
+    using at_start_in_happ_seqE' assms by blast
+  hence "(s + d, at_end a) \<in> happ_seq" unfolding plan_happ_seq_def by blast
+  with durations_positive[simplified durations_positive_def] as_in_plan not_ended 
+  have t_sd: "t \<le> s + d" by fastforce
+  
+  from snap_in_B
+  obtain d' where
+    at_in_plan: "(a, t, d') \<in> ran \<pi>" 
+    using at_start_in_happ_seqE' assms by blast
+
+  from started as_in_plan t_sd at_in_plan
+  show False using no_self_overlap[THEN no_self_overlap_spec] by fastforce
+qed
+
+lemma executing_when_ending:
+  assumes snap_in_B: "(at_end a) \<in> B t"
+      and a_in_actions: "a \<in> actions"
+      and no_self_overlap: nso_\<pi>
+      and durations_positive: dp_\<pi>
+      and plan_actions_in_problem: pap_\<pi>
+    shows "a \<in> ES t"
+proof -
+  from snap_in_B
+  obtain s d where
+    s: "(a, s, d) \<in> ran \<pi>"   
+    "t = s + d"
+    using at_end_in_happ_seqE' assms by blast
+  with durations_positive[simplified durations_positive_def] 
+  have "(s, at_start a) \<in> happ_seq \<and> s < t" unfolding plan_happ_seq_def by auto
+  moreover
+  have "\<not>(\<exists>s'. (s', at_end a) \<in> happ_seq \<and> s \<le> s' \<and> s' < t)"
+  proof (rule notI)
+    assume "\<exists>s'. (s', at_end a) \<in> happ_seq \<and> s \<le> s' \<and> s' < t"
+    then obtain s' where
+      s': "(s', at_end a) \<in> happ_seq" 
+      "s \<le> s' \<and> s' < t" by auto
+  
+    then obtain \<tau> \<epsilon> where
+      \<tau>: "(a, \<tau>, \<epsilon>) \<in> ran \<pi>"
+      "s' = \<tau> + \<epsilon>"
+      using at_end_in_happ_seqE' assms by blast
+
+    hence "(\<tau>, at_start a) \<in> happ_seq" unfolding plan_happ_seq_def by blast
+
+    consider "\<tau> \<le> s" | "s \<le> \<tau>" by fastforce
+    thus False
+    proof cases
+      case 1
+      with s'(2) s(2) \<tau>(2)
+      have "\<tau> = s \<longrightarrow> \<epsilon> \<noteq> d" by blast
+      with no_self_overlap[THEN no_self_overlap_spec, OF \<tau>(1) s(1)] 1 s'(2) \<tau>(2) 
+      show ?thesis by blast
+    next
+      case 2
+      from \<open>s \<le> s' \<and> s' < t\<close>[simplified \<open>t = s + d\<close> \<open>s' = \<tau> + \<epsilon>\<close>] 
+        durations_positive[simplified durations_positive_def] \<open>(a, \<tau>, \<epsilon>) \<in> ran \<pi>\<close>
+      have "\<tau> \<le> s + d" by (meson less_add_same_cancel1 order_le_less_trans order_less_imp_le)
+      moreover
+      from 2 s'(2) s(2) \<tau>(2)
+      have "\<tau> = s \<longrightarrow> \<epsilon> \<noteq> d" by blast
+      ultimately 
+      show ?thesis using 2 no_self_overlap[THEN no_self_overlap_spec, OF s(1) \<tau>(1)] by blast
+    qed
+  qed
+  ultimately
+  show ?thesis unfolding exec_state_sequence_def using a_in_actions by blast
+qed
+
+lemma execution_state_unchanging:
+  assumes not_starting: "at_start a \<notin> B t"
+      and not_ending:   "at_end a \<notin> B t"
+    shows "a \<in> ES t \<longleftrightarrow> a \<in> IES t"
+proof (rule iffI)
+  assume "a \<in> ES t"
+  with exec_state_sequence_def
+  obtain s where
+    s: "a \<in> actions \<and> (s, at_start a) \<in> happ_seq \<and> s < t" 
+    and s': "(\<nexists>s'. (s', at_end a) \<in> happ_seq \<and> s \<le> s' \<and> s' < t)" by blast
+  have "s \<le> t" using s by auto
+  moreover
+  have "(\<nexists>s'. (s', at_end a) \<in> happ_seq \<and> s \<le> s' \<and> s' \<le> t)" using s' not_ending by auto
+  ultimately
+  show "a \<in> IES t" using s unfolding exec_state_sequence'_def by blast
+next
+  assume "a \<in> IES t"
+  with exec_state_sequence'_def
+  obtain s where  
+    s: "a \<in> actions \<and> (s, at_start a) \<in> happ_seq \<and> s \<le> t" 
+    and s': "(\<nexists>s'. (s', at_end a) \<in> happ_seq \<and> s \<le> s' \<and> s' \<le> t)" by blast
+  have "s < t" using not_starting s by force
+  moreover 
+  have "(\<nexists>s'. (s', at_end a) \<in> happ_seq \<and> s \<le> s' \<and> s' < t)" using s' by auto
+  ultimately
+  show "a \<in> ES t" using s unfolding exec_state_sequence_def by blast
+qed
+
+  
+
+end
+end
